Check permission and locality of entry points in LR

theories/examples/switcher/switcher.v
@@ -160,9 +160,12 @@ Section Switcher.
         (b_switcher + (1 + length switcher_call_instrs) )%a = Some a_switcher_return ;
       }.
 
-  Definition is_switcher_entry_point `{switcherLayout} (b e a : Addr) :=
-    if (b =? b_switcher)%a && (e =? e_switcher)%a
-    then (if (a =? a_switcher_call)%a || (a =? a_switcher_return)%a then true else false)
+  Definition is_switcher_entry_point `{switcherLayout} (p : Perm) (g : Locality) (b e a : Addr) :=
+    if (bool_decide (p = XSRW_)) && (bool_decide (g = Local))
+    then
+      if (b =? b_switcher)%a && (e =? e_switcher)%a
+      then (if (a =? a_switcher_call)%a || (a =? a_switcher_return)%a then true else false)
+      else false
     else false.
 
 End Switcher.
